Refactor lemmas mostly and finish some proofs for normaliation
Commented out some lemmas which didn't make sense or weren't necessary, at
least for the normalization theorem.
Finished some proofs required for the normalization theorem.
Delete ordType references and left everything compiling.

src/Graph.v
@@ -5,6 +5,7 @@ Unset Printing Implicit Defensive.
 
 From CoqUtils Require Import string.
 
+Require Import Base.
 
 Section GraphQLGraph.
 
@@ -45,7 +46,7 @@ Section GraphQLGraph.
       Fields and values).
    *)
   Record node := Node {
-                    ntype : string;
+                    ntype : Name;
                     nfields : seq (fld * (Vals + seq Vals)%type)  (* Vals could include list values? *)
                   }.
 
