src/theory/GraphConformanceLemmas.v
@@ -3,9 +3,8 @@ Set Implicit Arguments.
 Unset Strict Implicit.
 Unset Printing Implicit Defensive.
 
-From extructures Require Import ord fset fmap.
-
-
+From CoqUtils Require Import string.
+Require Import Base.
 Require Import Schema.
 Require Import SchemaWellFormedness.
 Require Import SchemaAux.
@@ -19,13 +18,13 @@ Require Import SeqExtra.
 
 Section Theory.
 
-  Variables (N Name Vals: ordType).
+  Variables (Vals: eqType).
 
-  Variable (s : @wfSchema Name Vals) (g : conformedGraph s).
+  Variable (s : @wfGraphQLSchema Vals) (g : conformedGraph s).
 
   
   Lemma argument_conformsP ty fname arg :
-    reflect (exists2 fld_arg, lookup_argument_in_type_and_field s ty fname arg.1 = Some fld_arg & s.(hasType) fld_arg.(argtype) arg.2)
+    reflect (exists2 fld_arg, lookup_argument_in_type_and_field s ty fname arg.1 = Some fld_arg & s.(has_type) fld_arg.(argtype) arg.2)
             (argument_conforms s ty fname arg).
   Proof.
     apply: (iffP idP); rewrite /argument_conforms; case: arg => argname value.
@@ -36,25 +35,25 @@ Section Theory.
 
   
   Lemma nodes_have_object_typeP graph :
-    reflect (forall node, node \in graph.(nodes) -> is_object_type s node.(type))
+    reflect (forall node, node \in graph.(nodes) -> is_object_type s node.(ntype))
             (nodes_have_object_type s graph).
   Proof. by apply: (iffP allP). Qed.
 
 
   
   Lemma aux_root_query_type graph :
-    root_type_conforms s graph -> graph.(root).(type) = s.(query_type).
+    root_type_conforms s graph -> graph.(root).(ntype) = s.(query_type).
   Proof. by rewrite /root_type_conforms; move/eqP. Qed.
   
   Lemma root_query_type :
-    g.(root).(type) = s.(query_type).
+    g.(root).(ntype) = s.(query_type).
   Proof.
     case: g => g' H *.
       by move: (aux_root_query_type H).
   Qed.
 
   Lemma node_in_graph_has_object_type :
-    forall u, u \in g.(nodes) -> is_object_type s u.(type).
+    forall u, u \in g.(nodes) -> is_object_type s u.(ntype).
   Proof.
     apply/nodes_have_object_typeP.
     by case: g.
@@ -63,9 +62,9 @@ Section Theory.
   
 
   Lemma neighbours_are_subtype_of_field u fld fdef  :
-    lookup_field_in_type s u.(type) fld.(label) = Some fdef ->
+    lookup_field_in_type s u.(ntype) fld.(label) = Some fdef ->
     forall v, v \in neighbours_with_field g u fld ->
-               v.(type) \in get_possible_types s fdef.(return_type).
+               v.(ntype) \in get_possible_types s fdef.(return_type).
   Proof.
     move=> Hlook.
     case: g => g' Hroot Hedges.
