src/theory/QueryConformanceLemmas.v
@@ -4,9 +4,9 @@ Unset Strict Implicit.
 Unset Printing Implicit Defensive.
 
 From Equations Require Import Equations.
+From CoqUtils Require Import string.
 
-From extructures Require Import ord fset fmap.
-
+Require Import Base.
 Require Import Schema.
 Require Import SchemaAux.
 Require Import SchemaAuxLemmas.
@@ -24,7 +24,7 @@ Require Import Ssromega.
 
 
 Section Theory.
-  Transparent qname qresponse_name.
+  Transparent qresponse_name.
 
 
   Ltac apply_and3P := apply/and3P; split=> //.
@@ -33,11 +33,11 @@ Section Theory.
   Ltac query_conforms := simp query_conforms; try move/and5P; try apply/and5P.
 
 
-  Variables (Name Vals : ordType).
+  Variables (Vals : eqType).
   
   Section FragmentSpread.
 
-    Variable (s : @wfSchema Name Vals).
+    Variable (s : @wfGraphQLSchema Vals).
     
     (* TODO: rename **)
     Lemma object_spreads_E parent_type ty :
@@ -160,208 +160,209 @@ Section Theory.
 
   Section QueryConformance.
 
-    Variable (s : @wfSchema Name Vals).
+    (* Variable (s : @wfSchema Name Vals). *)
     
-    Lemma queries_conform_inv ty φ :
-      all (query_conforms s ty) φ ->
-      have_compatible_response_shapes s ty φ ->
-      is_field_merging_possible s ty φ ->
-      queries_conform s ty φ.
-    Proof.
-        by intros; rewrite /queries_conform; apply/and3P; split.
-    Qed.
-    
-    
-
-    Lemma found_fields_with_response_name_share_field_name_in_obj ty rname φ :
-      is_object_type s ty ->
-      is_field_merging_possible s ty φ ->
-      forall fname,
-        all (has_field_name fname) (find_queries_with_label s rname ty φ).
-    Proof.
-      elim: φ => //=; case=> [f α | l f α | f α β | l f α β | t β] φ IH Hscope; simp is_field_merging_possible.
-
-      - rewrite Hscope /=; simp are_equivalent => /andP [Hequiv Hmerge] fname.
-    Admitted.
-
-
-
-    
-    Lemma nf_conformsP type_in_scope f α φ :
-      reflect (exists2 fld, lookup_field_in_type s type_in_scope f = Some fld &
-                            [&& (is_object_type s fld.(return_type) || is_abstract_type s fld.(return_type)),
-                             arguments_conform s fld.(fargs) α,
-                             φ != [::] &
-                             all (query_conforms s fld.(return_type)) φ])
-              (query_conforms s type_in_scope (NestedField f α φ)).
-    Proof.
-      apply: (iffP idP).
-      - simp query_conforms.
-        case Hlook : lookup_field_in_type => [fld |] //= H.
-          by exists fld.
-               - move=> [fld Hlook H].
-                   by simp query_conforms; rewrite Hlook. 
-    Qed.
-
-    Lemma nlf_conformsP type_in_scope l f α φ :
-      reflect (exists2 fld, lookup_field_in_type s type_in_scope f = Some fld &
-                            [&& (is_object_type s fld.(return_type) || is_abstract_type s fld.(return_type)),
-                             arguments_conform s fld.(fargs) α,
-                             φ != [::] &
-                             all (query_conforms s fld.(return_type)) φ])
-              (query_conforms s type_in_scope (NestedLabeledField l f α φ)).
-    Proof.
-      apply: (iffP idP).
-      - simp query_conforms.
-        case Hlook : lookup_field_in_type => [fld |] // H.
-          by exists fld.
-               - move=> [fld Hlook H].
-                   by simp query_conforms; rewrite Hlook. 
-    Qed.
-
-    
-    Lemma scope_is_obj_or_abstract_for_field ty q :
-      is_field q ->
-      query_conforms s ty q ->
-      is_object_type s ty \/ is_interface_type s ty.
-    Proof.
-      case: q => //= [f α | l f α | f α φ | l f α φ] _; simp query_conforms;
-                  case Hlook: lookup_field_in_type => [fld|] // _;
-                                                       have H: lookup_field_in_type s ty f by rewrite /isSome Hlook.
-
-      all: by apply: (lookup_field_in_type_is_obj_or_intf H).
-    Qed.
-    
-    Lemma nested_field_is_obj_or_abstract ty n α ϕ :
-      query_conforms s ty (NestedField n α ϕ) ->
-      is_object_type s ty \/ is_interface_type s ty.
-    Proof.
-      simp query_conforms.
-      case Hlook: lookup_field_in_type => [fld|] // _.
-      have H: lookup_field_in_type s ty n by rewrite /isSome Hlook.
-        by apply: (lookup_field_in_type_is_obj_or_intf H).
-    Qed.
-
-    Lemma scope_is_obj_or_abstract_for_nlf ty l f α φ :
-      query_conforms s ty (NestedLabeledField l f α φ) ->
-      is_object_type s ty \/ is_interface_type s ty.
-    Proof.
-      simp query_conforms.
-      case Hlook: lookup_field_in_type => [fld|] // _.
-      have H: lookup_field_in_type s ty f by rewrite /isSome Hlook.
-        by apply: (lookup_field_in_type_is_obj_or_intf H).
-    Qed.
-
+    (* Lemma queries_conform_inv ty φ : *)
+    (*   all (query_conforms s ty) φ -> *)
+    (*   have_compatible_response_shapes s ty φ -> *)
+    (*   is_field_merging_possible s ty φ -> *)
+    (*   queries_conform s ty φ. *)
+    (* Proof. *)
+    (*     by intros; rewrite /queries_conform; apply/and3P; split. *)
+    (* Qed. *)
     
     
-    Lemma type_in_scope_N_scalar_enum :
-      forall type_in_scope ϕ,
-        query_conforms s type_in_scope ϕ ->
-        [\/ is_object_type s type_in_scope,
-         is_interface_type s type_in_scope |
-         is_union_type s type_in_scope].
-    Proof.
-      move=> ty.
-      case=> [f α |  l f α |  f α ϕ |  l f α ϕ |  t ϕ]; simp query_conforms.
-      all: do ?[case Hlook: lookup_field_in_type => [fld|] //= _;
-                                                   have H: lookup_field_in_type ty f by rewrite /isSome Hlook].
-      all: do ?[by move: (lookup_field_in_type_is_obj_or_intf H) => [Hobj | Hint]; [constructor 1 | constructor 2] ].
+
+    (* Lemma found_fields_with_response_name_share_field_name_in_obj ty rname φ : *)
+    (*   is_object_type s ty -> *)
+    (*   is_field_merging_possible s ty φ -> *)
+    (*   forall fname, *)
+    (*     all (has_field_name fname) (find_queries_with_label s rname ty φ). *)
+    (* Proof. *)
+    (*   elim: φ => //=; case=> [f α | l f α | f α β | l f α β | t β] φ IH Hscope; simp is_field_merging_possible. *)
+
+    (*   - rewrite Hscope /=; simp are_equivalent => /andP [Hequiv Hmerge] fname. *)
+    (* Admitted. *)
+
+
+
+    
+    (* Lemma nf_conformsP type_in_scope f α φ : *)
+    (*   reflect (exists2 fld, lookup_field_in_type s type_in_scope f = Some fld & *)
+    (*                         [&& (is_object_type s fld.(return_type) || is_abstract_type s fld.(return_type)), *)
+    (*                          arguments_conform s fld.(fargs) α, *)
+    (*                          φ != [::] & *)
+    (*                          all (query_conforms s fld.(return_type)) φ]) *)
+    (*           (query_conforms s type_in_scope (NestedField f α φ)). *)
+    (* Proof. *)
+    (*   apply: (iffP idP). *)
+    (*   - simp query_conforms. *)
+    (*     case Hlook : lookup_field_in_type => [fld |] //= H. *)
+    (*       by exists fld. *)
+    (*            - move=> [fld Hlook H]. *)
+    (*                by simp query_conforms; rewrite Hlook.  *)
+    (* Qed. *)
+
+    (* Lemma nlf_conformsP type_in_scope l f α φ : *)
+    (*   reflect (exists2 fld, lookup_field_in_type s type_in_scope f = Some fld & *)
+    (*                         [&& (is_object_type s fld.(return_type) || is_abstract_type s fld.(return_type)), *)
+    (*                          arguments_conform s fld.(fargs) α, *)
+    (*                          φ != [::] & *)
+    (*                          all (query_conforms s fld.(return_type)) φ]) *)
+    (*           (query_conforms s type_in_scope (NestedLabeledField l f α φ)). *)
+    (* Proof. *)
+    (*   apply: (iffP idP). *)
+    (*   - simp query_conforms. *)
+    (*     case Hlook : lookup_field_in_type => [fld |] // H. *)
+    (*       by exists fld. *)
+    (*            - move=> [fld Hlook H]. *)
+    (*                by simp query_conforms; rewrite Hlook.  *)
+    (* Qed. *)
+
+    
+    (* Lemma scope_is_obj_or_abstract_for_field ty q : *)
+    (*   is_field q -> *)
+    (*   query_conforms s ty q -> *)
+    (*   is_object_type s ty \/ is_interface_type s ty. *)
+    (* Proof. *)
+    (*   case: q => //= [f α | l f α | f α φ | l f α φ] _; simp query_conforms; *)
+    (*               case Hlook: lookup_field_in_type => [fld|] // _; *)
+    (*                                                    have H: lookup_field_in_type s ty f by rewrite /isSome Hlook. *)
+
+    (*   all: by apply: (lookup_field_in_type_is_obj_or_intf H). *)
+    (* Qed. *)
+    
+    (* Lemma nested_field_is_obj_or_abstract ty n α ϕ : *)
+    (*   query_conforms s ty (NestedField n α ϕ) -> *)
+    (*   is_object_type s ty \/ is_interface_type s ty. *)
+    (* Proof. *)
+    (*   simp query_conforms. *)
+    (*   case Hlook: lookup_field_in_type => [fld|] // _. *)
+    (*   have H: lookup_field_in_type s ty n by rewrite /isSome Hlook. *)
+    (*     by apply: (lookup_field_in_type_is_obj_or_intf H). *)
+    (* Qed. *)
+
+    (* Lemma scope_is_obj_or_abstract_for_nlf ty l f α φ : *)
+    (*   query_conforms s ty (NestedLabeledField l f α φ) -> *)
+    (*   is_object_type s ty \/ is_interface_type s ty. *)
+    (* Proof. *)
+    (*   simp query_conforms. *)
+    (*   case Hlook: lookup_field_in_type => [fld|] // _. *)
+    (*   have H: lookup_field_in_type s ty f by rewrite /isSome Hlook. *)
+    (*     by apply: (lookup_field_in_type_is_obj_or_intf H). *)
+    (* Qed. *)
+
+    
+    
+  (*   Lemma type_in_scope_N_scalar_enum : *)
+  (*     forall type_in_scope ϕ, *)
+  (*       query_conforms s type_in_scope ϕ -> *)
+  (*       [\/ is_object_type s type_in_scope, *)
+  (*        is_interface_type s type_in_scope | *)
+  (*        is_union_type s type_in_scope]. *)
+  (*   Proof. *)
+  (*     move=> ty. *)
+  (*     case=> [f α |  l f α |  f α ϕ |  l f α ϕ |  t ϕ]; simp query_conforms. *)
+  (*     all: do ?[case Hlook: lookup_field_in_type => [fld|] //= _; *)
+  (*                                                  have H: lookup_field_in_type ty f by rewrite /isSome Hlook]. *)
+  (*     all: do ?[by move: (lookup_field_in_type_is_obj_or_intf H) => [Hobj | Hint]; [constructor 1 | constructor 2] ]. *)
       
-    (*
-    case Hlook: lookup_type => [tdef|] //.
-    by case: tdef Hlook => //=; do ?[rewrite fset0I //=];
-                         [constructor 1; simp is_object_type
-                         | constructor 2; simp is_interface_type
-                         | constructor 3; simp is_union_type]; rewrite Hlook.
+  (*   (* *)
+  (*   case Hlook: lookup_type => [tdef|] //. *)
+  (*   by case: tdef Hlook => //=; do ?[rewrite fset0I //=]; *)
+  (*                        [constructor 1; simp is_object_type *)
+  (*                        | constructor 2; simp is_interface_type *)
+  (*                        | constructor 3; simp is_union_type]; rewrite Hlook. *)
     
-    by rewrite fset0I /=.
-  Qed.*)
-    Admitted.
+  (*   by rewrite fset0I /=. *)
+  (* Qed.*) *)
+  (*   Admitted. *)
 
-    Lemma type_in_scope_N_scalar type_in_scope φ :
-      query_conforms s type_in_scope φ ->
-      is_scalar_type s type_in_scope = false.
-    Admitted.
+    (* Lemma type_in_scope_N_scalar type_in_scope φ : *)
+    (*   query_conforms s type_in_scope φ -> *)
+    (*   is_scalar_type s type_in_scope = false. *)
+    (* Admitted. *)
 
-    Lemma type_in_scope_N_enum type_in_scope φ :
-      query_conforms s type_in_scope φ ->
-      is_enum_type s type_in_scope = false.
-    Admitted.
-
-    
-    Lemma type_in_scope_N_obj_is_abstract type_in_scope φ :
-      query_conforms s type_in_scope φ ->
-      is_object_type s type_in_scope = false ->
-      is_abstract_type s type_in_scope.
-    Proof.
-        by move/type_in_scope_N_scalar_enum => [-> | Hintf | Hunion ] _ //; rewrite /is_abstract_type; apply/orP; [left | right].
-    Qed.
-    
-    Lemma queries_conform_obj_int_union type_in_scope ϕ :
-      ϕ != [::] ->
-      queries_conform s type_in_scope ϕ ->
-      [\/ is_object_type s type_in_scope,
-       is_interface_type s type_in_scope |
-       is_union_type s type_in_scope].
-    Proof.
-      rewrite /queries_conform.
-      case: ϕ => //= hd tl _.
-      move/andP => [/andP [Hqc Hqsc] _].
-      apply (type_in_scope_N_scalar_enum Hqc).
-    Qed.
-
-    Lemma nlf_conforms_lookup_some ty l n α ϕ :
-      query_conforms s ty (NestedLabeledField l n α ϕ) ->
-      exists fld, lookup_field_in_type s ty n = Some fld.
-    Proof. simp query_conforms.
-      case Hlook : lookup_field_in_type => [fld'|] //.
-        by exists fld'.
-    Qed.
-
-    Lemma queries_conform_int_impl ty ti qs :
-      ty \in implementation s ti ->
-             all (@is_field Name Vals) qs ->
-             queries_conform s ti qs ->       
-             queries_conform s ty qs.
-    Proof.
-      move=> Himpl Hflds.
-      rewrite /queries_conform.
-      move/andP=> [/allP Hqsc Hmerge].
-      apply/andP; split=> //.
-      apply/allP.
-      move=> x Hin.
-      move: (Hqsc x Hin) => {Hin}.
-      case: x => //; [move=> f α | move=> l f α | move=> f α ϕ | move=> l f α ϕ | move=> t ϕ];
-                  simp query_conforms; do ? rewrite (field_in_interface_in_object f Himpl);
-                    do ? case lookup_field_in_type => //.
-      - Admitted. (* Invalid case - all fields *)
-
+    (* Lemma type_in_scope_N_enum type_in_scope φ : *)
+    (*   query_conforms s type_in_scope φ -> *)
+    (*   is_enum_type s type_in_scope = false. *)
+    (* Admitted. *)
 
     
+    (* Lemma type_in_scope_N_obj_is_abstract type_in_scope φ : *)
+    (*   query_conforms s type_in_scope φ -> *)
+    (*   is_object_type s type_in_scope = false -> *)
+    (*   is_abstract_type s type_in_scope. *)
+    (* Proof. *)
+    (*     by move/type_in_scope_N_scalar_enum => [-> | Hintf | Hunion ] _ //; rewrite /is_abstract_type; apply/orP; [left | right]. *)
+    (* Qed. *)
 
-    Lemma sf_conforms_in_interface_in_obj ti tyo f α :
-      tyo \in implementation s ti ->
-              query_conforms s ti (SingleField f α) ->
-              query_conforms s tyo (SingleField f α).
-    Proof.
-      move=> Hin.
-      simp query_conforms.
-      case Hlook : lookup_field_in_type => [fld |] //= /andP [Hty Hα].
-      move: (in_implementation_is_object Hin) => Hobj.
-      move: (field_in_interface_in_object_same_return_type Hin Hlook) => [fld' Hlook' Hrty].
-      rewrite Hlook' /= -Hrty.
-      apply/andP; split => //.
-      move: Hα; rewrite /arguments_conform.
-      move/allP=> Hα.
-      apply/allP=> arg Hain.
-      move: (Hα arg Hain) => {Hα Hain}.
-      case: arg => n v.
-      have: lookup_field_in_type s ti f = Some fld -> fld \in fields s ti.
-      move: (has_implementation_is_interface Hin) => /is_interface_type_E.
-      case=> [i [flds Hilook] ].
+    
+    (* Lemma queries_conform_obj_int_union type_in_scope ϕ : *)
+    (*   ϕ != [::] -> *)
+    (*   queries_conform s type_in_scope ϕ -> *)
+    (*   [\/ is_object_type s type_in_scope, *)
+    (*    is_interface_type s type_in_scope | *)
+    (*    is_union_type s type_in_scope]. *)
+    (* Proof. *)
+    (*   rewrite /queries_conform. *)
+    (*   case: ϕ => //= hd tl _. *)
+    (*   move/andP => [/andP [Hqc Hqsc] _]. *)
+    (*   apply (type_in_scope_N_scalar_enum Hqc). *)
+    (* Qed. *)
+
+    (* Lemma nlf_conforms_lookup_some ty l n α ϕ : *)
+    (*   query_conforms s ty (NestedLabeledField l n α ϕ) -> *)
+    (*   exists fld, lookup_field_in_type s ty n = Some fld. *)
+    (* Proof. simp query_conforms. *)
+    (*   case Hlook : lookup_field_in_type => [fld'|] //. *)
+    (*     by exists fld'. *)
+    (* Qed. *)
+
+    (* Lemma queries_conform_int_impl ty ti qs : *)
+    (*   ty \in implementation s ti -> *)
+    (*          all (@is_field Name Vals) qs -> *)
+    (*          queries_conform s ti qs ->        *)
+    (*          queries_conform s ty qs. *)
+    (* Proof. *)
+    (*   move=> Himpl Hflds. *)
+    (*   rewrite /queries_conform. *)
+    (*   move/andP=> [/allP Hqsc Hmerge]. *)
+    (*   apply/andP; split=> //. *)
+    (*   apply/allP. *)
+    (*   move=> x Hin. *)
+    (*   move: (Hqsc x Hin) => {Hin}. *)
+    (*   case: x => //; [move=> f α | move=> l f α | move=> f α ϕ | move=> l f α ϕ | move=> t ϕ]; *)
+    (*               simp query_conforms; do ? rewrite (field_in_interface_in_object f Himpl); *)
+    (*                 do ? case lookup_field_in_type => //. *)
+    (*   - Admitted. (* Invalid case - all fields *) *)
+
+
+    
+
+    (* Lemma sf_conforms_in_interface_in_obj ti tyo f α : *)
+    (*   tyo \in implementation s ti -> *)
+    (*           query_conforms s ti (SingleField f α) -> *)
+    (*           query_conforms s tyo (SingleField f α). *)
+    (* Proof. *)
+    (*   move=> Hin. *)
+    (*   simp query_conforms. *)
+    (*   case Hlook : lookup_field_in_type => [fld |] //= /andP [Hty Hα]. *)
+    (*   move: (in_implementation_is_object Hin) => Hobj. *)
+    (*   move: (field_in_interface_in_object_same_return_type Hin Hlook) => [fld' Hlook' Hrty]. *)
+    (*   rewrite Hlook' /= -Hrty. *)
+    (*   apply/andP; split => //. *)
+    (*   move: Hα; rewrite /arguments_conform. *)
+    (*   move/allP=> Hα. *)
+    (*   apply/allP=> arg Hain. *)
+    (*   move: (Hα arg Hain) => {Hα Hain}. *)
+    (*   case: arg => n v. *)
+    (*   have: lookup_field_in_type s ti f = Some fld -> fld \in fields s ti. *)
+    (*   move: (has_implementation_is_interface Hin) => /is_interface_type_E. *)
+    (*   case=> [i [flds Hilook] ]. *)
       
-      rewrite /fields /lookup_field_in_type Hilook.
-    Admitted.
+    (*   rewrite /fields /lookup_field_in_type Hilook. *)
+    (* Admitted. *)
 
     
   End QueryConformance.
